CDCL(T): reuse incremental

Weidenbach_Book/CDCL/CDCL_W_Incremental.thy
@@ -178,7 +178,7 @@ text \<open>This invariant holds all the invariant related to the strategy. See 
 
 text \<open>When we add a new clause, we reduce the trail until we get to tho first literal included in C.
   Then we can mark the conflict.\<close>
-fun cut_trail_wrt_clause where
+fun (in state\<^sub>W) cut_trail_wrt_clause where
 "cut_trail_wrt_clause C [] S = S" |
 "cut_trail_wrt_clause C (Decided L # M) S =
   (if -L \<in># C then S
@@ -187,26 +187,29 @@ fun cut_trail_wrt_clause where
   (if -L \<in># C then S
     else cut_trail_wrt_clause C M (tl_trail S))"
 
-definition add_new_clause_and_update :: "'v clause \<Rightarrow> 'st \<Rightarrow> 'st" where
-"add_new_clause_and_update C S =
-  (if trail S \<Turnstile>as CNot C
-  then update_conflicting (Some C) (add_init_cls C
-    (cut_trail_wrt_clause C (trail S) S))
-  else add_init_cls C S)"
+definition (in state\<^sub>W) reduce_trail_wrt_clause :: "'v clause \<Rightarrow> 'st \<Rightarrow> 'st" where
+"reduce_trail_wrt_clause C S = update_conflicting (Some C) (cut_trail_wrt_clause C (trail S) S)"
 
-lemma init_clss_cut_trail_wrt_clause[simp]:
+definition add_new_clause_and_update :: "'v clause \<Rightarrow> 'st \<Rightarrow> 'st" where
+"add_new_clause_and_update C S = reduce_trail_wrt_clause C (add_init_cls C S)"
+
+lemma (in state\<^sub>W) init_clss_cut_trail_wrt_clause[simp]:
   "init_clss (cut_trail_wrt_clause C M S) = init_clss S"
   by (induction rule: cut_trail_wrt_clause.induct) auto
 
-lemma learned_clss_cut_trail_wrt_clause[simp]:
+lemma (in state\<^sub>W) learned_clss_cut_trail_wrt_clause[simp]:
   "learned_clss (cut_trail_wrt_clause C M S) = learned_clss S"
   by (induction rule: cut_trail_wrt_clause.induct) auto
 
-lemma conflicting_clss_cut_trail_wrt_clause[simp]:
+lemma (in state\<^sub>W) conflicting_clss_cut_trail_wrt_clause[simp]:
   "conflicting (cut_trail_wrt_clause C M S) = conflicting S"
   by (induction rule: cut_trail_wrt_clause.induct) auto
 
-lemma trail_cut_trail_wrt_clause:
+lemma (in state\<^sub>W) clauses_cut_trail_wrt_clause[simp]:
+  "clauses (cut_trail_wrt_clause C M S) = clauses S"
+  by (auto simp: clauses_def)
+
+lemma (in state\<^sub>W) trail_cut_trail_wrt_clause:
   "\<exists>M.  trail S = M @ trail (cut_trail_wrt_clause C (trail S) S)"
 proof (induction "trail S" arbitrary: S rule: ann_lit_list_induct)
   case Nil
@@ -219,7 +222,7 @@ next
   then show ?case using Cons_eq_appendI by fastforce+
 qed
 
-lemma n_dup_no_dup_trail_cut_trail_wrt_clause[simp]:
+lemma (in state\<^sub>W) n_dup_no_dup_trail_cut_trail_wrt_clause[simp]:
   assumes n_d: "no_dup (trail T)"
   shows "no_dup (trail (cut_trail_wrt_clause C (trail T) T))"
 proof -
@@ -230,7 +233,19 @@ proof -
     using n_d unfolding arg_cong[OF M, of no_dup] by (auto simp: no_dup_def)
 qed
 
-lemma cut_trail_wrt_clause_CNot_trail:
+
+lemma trail_cut_trail_wrt_clause_mono:
+  \<open>trail S = trail T \<Longrightarrow> trail (cut_trail_wrt_clause C M S) =
+  trail (cut_trail_wrt_clause C M T)\<close>
+  by (induction M arbitrary: T S rule: ann_lit_list_induct) auto
+
+lemma trail_cut_trail_wrt_clause_add_init_cls[simp]:
+  \<open>trail (cut_trail_wrt_clause C M (add_init_cls C S)) =
+  trail (cut_trail_wrt_clause C M S)\<close>
+    by (subst trail_cut_trail_wrt_clause_mono)
+      auto
+
+lemma (in state\<^sub>W) cut_trail_wrt_clause_CNot_trail:
   assumes "trail T \<Turnstile>as CNot C"
   shows
     "(trail ((cut_trail_wrt_clause C (trail T) T))) \<Turnstile>as CNot C"
@@ -279,7 +294,7 @@ next
     qed
 qed
 
-lemma cut_trail_wrt_clause_hd_trail_in_or_empty_trail:
+lemma (in state\<^sub>W) cut_trail_wrt_clause_hd_trail_in_or_empty_trail:
   "((\<forall>L \<in>#C. -L \<notin> lits_of_l (trail T)) \<and> trail (cut_trail_wrt_clause C (trail T) T) = [])
     \<or> (-lit_of (hd (trail (cut_trail_wrt_clause C (trail T) T))) \<in># C
        \<and> length (trail (cut_trail_wrt_clause C (trail T) T)) \<ge> 1)"
@@ -295,23 +310,24 @@ next
 qed
 
 text \<open>The following function allows to mark a conflict while backtrack at the correct position.\<close>
-inductive cdcl\<^sub>W_OOO_conflict :: \<open>'st \<Rightarrow> 'st \<Rightarrow> bool\<close> for S :: 'st where
+inductive (in state\<^sub>W)cdcl\<^sub>W_OOO_conflict :: \<open>'st \<Rightarrow> 'st \<Rightarrow> bool\<close> for S :: 'st where
 cdcl\<^sub>W_OOO_conflict_rule: \<open>cdcl\<^sub>W_OOO_conflict S T\<close>
 if
   \<open>trail S \<Turnstile>as CNot C\<close> and
   \<open>C \<in># clauses S\<close> and
   \<open>conflicting S = None\<close>
-  \<open>T \<sim> add_new_clause_and_update C S\<close>
+  \<open>T \<sim> reduce_trail_wrt_clause C S\<close>
 
-lemma cdcl\<^sub>W_all_struct_inv_add_new_clause_and_update_cdcl\<^sub>W_all_struct_inv:
+lemma (in conflict_driven_clause_learning\<^sub>W)
+     cdcl\<^sub>W_all_struct_inv_add_new_clause_and_update_cdcl\<^sub>W_all_struct_inv:
   assumes
     inv_T: "cdcl\<^sub>W_all_struct_inv T" and
     tr_C[simp]: "trail T \<Turnstile>as CNot C" and
-    [simp]: "distinct_mset C"
-  shows "cdcl\<^sub>W_all_struct_inv (add_new_clause_and_update C T)" (is "cdcl\<^sub>W_all_struct_inv ?T'")
+    [simp]: "distinct_mset C" and
+    C: \<open>C \<in># clauses T\<close>
+  shows "cdcl\<^sub>W_all_struct_inv (reduce_trail_wrt_clause C T)" (is "cdcl\<^sub>W_all_struct_inv ?T'")
 proof -
-  let ?T = "update_conflicting (Some C)
-    (add_init_cls C (cut_trail_wrt_clause C (trail T) T))"
+  let ?T = "update_conflicting (Some C) ((cut_trail_wrt_clause C (trail T) T))"
   obtain M where
     M: "trail T = M @ trail (cut_trail_wrt_clause C (trail T) T)"
       using trail_cut_trail_wrt_clause[of T "C"] by blast
@@ -327,8 +343,10 @@ proof -
   using inv_T arg_cong[OF M, of get_all_mark_of_propagated] by auto
 
   have [simp]: "no_strange_atm ?T"
-    using inv_T unfolding cdcl\<^sub>W_all_struct_inv_def no_strange_atm_def add_new_clause_and_update_def
-    cdcl\<^sub>W_M_level_inv_def by (auto 20 1)
+    using inv_T C unfolding cdcl\<^sub>W_all_struct_inv_def no_strange_atm_def
+    cdcl\<^sub>W_M_level_inv_def reduce_trail_wrt_clause_def
+   by (auto dest!: multi_member_split[of C] simp: clauses_def, auto 20 1)
+
   have M_lev: "cdcl\<^sub>W_M_level_inv T"
     using inv_T unfolding cdcl\<^sub>W_all_struct_inv_def by blast
   then have "no_dup (M @ trail (cut_trail_wrt_clause C (trail T) T))"
@@ -383,35 +401,47 @@ proof -
     qed
 
   have [simp]: "cdcl\<^sub>W_learned_clause ?T"
-    using inv_T unfolding cdcl\<^sub>W_all_struct_inv_def cdcl\<^sub>W_learned_clause_alt_def
+    using inv_T C unfolding cdcl\<^sub>W_all_struct_inv_def cdcl\<^sub>W_learned_clause_alt_def
     by (auto dest!: H_proped simp: clauses_def)
   show ?thesis
-    using \<open>all_decomposition_implies_m (clauses ?T) (get_all_ann_decomposition (trail ?T))\<close>
-    unfolding cdcl\<^sub>W_all_struct_inv_def by (auto simp: add_new_clause_and_update_def)
+    using \<open>all_decomposition_implies_m (clauses ?T) (get_all_ann_decomposition (trail ?T))\<close> C
+    unfolding cdcl\<^sub>W_all_struct_inv_def
+    by (auto simp: reduce_trail_wrt_clause_def)
 qed
 
-lemma cdcl\<^sub>W_OOO_conflict_all_struct_invs:
+lemma (in conflict_driven_clause_learning\<^sub>W) cdcl\<^sub>W_OOO_conflict_is_conflict:
+  assumes \<open>cdcl\<^sub>W_OOO_conflict S U\<close>
+  shows \<open>conflict (cut_trail_wrt_clause (the (conflicting U)) (trail S) S) U\<close>
+  using assms by (auto simp: cdcl\<^sub>W_OOO_conflict.simps conflict.simps reduce_trail_wrt_clause_def
+      conj_disj_distribR ex_disj_distrib intro: cut_trail_wrt_clause_CNot_trail
+    dest!: multi_member_split)
+
+lemma (in conflict_driven_clause_learning\<^sub>W) cdcl\<^sub>W_OOO_conflict_all_struct_invs:
   assumes \<open>cdcl\<^sub>W_OOO_conflict S T\<close> and \<open>cdcl\<^sub>W_all_struct_inv S\<close>
   shows \<open>cdcl\<^sub>W_all_struct_inv T\<close>
   using assms(1)
 proof (cases rule: cdcl\<^sub>W_OOO_conflict.cases)
   case (cdcl\<^sub>W_OOO_conflict_rule C)
   then have \<open>distinct_mset C\<close>
-   using assms(2) unfolding cdcl\<^sub>W_all_struct_inv_def distinct_cdcl\<^sub>W_state_def
-   by (auto simp: clauses_def dest!: multi_member_split)
+    using assms(2) unfolding cdcl\<^sub>W_all_struct_inv_def distinct_cdcl\<^sub>W_state_def
+    by (auto simp: clauses_def dest!: multi_member_split)
+  then have \<open>cdcl\<^sub>W_all_struct_inv (reduce_trail_wrt_clause C S)\<close>
+    using cdcl\<^sub>W_all_struct_inv_add_new_clause_and_update_cdcl\<^sub>W_all_struct_inv[of S C]
+     cdcl\<^sub>W_all_struct_inv_cong[of T \<open>reduce_trail_wrt_clause C S\<close>] cdcl\<^sub>W_OOO_conflict_rule
+    by (auto simp: assms)
   then show ?thesis
-  using cdcl\<^sub>W_all_struct_inv_add_new_clause_and_update_cdcl\<^sub>W_all_struct_inv[of S C]
-   cdcl\<^sub>W_all_struct_inv_cong[of T \<open>add_new_clause_and_update C S\<close>] cdcl\<^sub>W_OOO_conflict_rule
-  by (auto simp: assms)
+    using cdcl\<^sub>W_all_struct_inv_cong[of T \<open>reduce_trail_wrt_clause C S\<close>] cdcl\<^sub>W_OOO_conflict_rule
+     cdcl\<^sub>W_OOO_conflict_is_conflict[OF assms(1)]
+    by (auto simp: assms)
 qed
 
-lemma get_maximum_level_Cons_notin:
+lemma (in -) get_maximum_level_Cons_notin:
   \<open>- lit_of L \<notin># C \<Longrightarrow> lit_of L \<notin># C \<Longrightarrow> get_maximum_level M C = get_maximum_level (L # M) C\<close>
   unfolding get_maximum_level_def
   by (subgoal_tac \<open>get_level (L # M) `# C = get_level M `# C\<close>)
    (auto intro!: image_mset_cong simp: get_level_cons_if atm_of_eq_atm_of)
 
-lemma backtrack_lvl_cut_trail_wrt_clause_get_maximum_level:
+lemma (in state\<^sub>W) backtrack_lvl_cut_trail_wrt_clause_get_maximum_level:
    \<open>M = trail S \<Longrightarrow> M \<Turnstile>as CNot D \<Longrightarrow> no_dup (trail S) \<Longrightarrow>
     backtrack_lvl (cut_trail_wrt_clause D M S) = get_maximum_level M D\<close>
   apply (induction D M S rule: cut_trail_wrt_clause.induct)
@@ -432,7 +462,7 @@ lemma backtrack_lvl_cut_trail_wrt_clause_get_maximum_level:
       split: if_splits)
   done
 
-lemma get_maximum_level_cut_trail_wrt_clause:
+lemma (in state\<^sub>W) get_maximum_level_cut_trail_wrt_clause:
    \<open>M = trail S \<Longrightarrow> M \<Turnstile>as CNot C \<Longrightarrow> no_dup (trail S) \<Longrightarrow>
     get_maximum_level (trail (cut_trail_wrt_clause C M S)) C =
            get_maximum_level M C\<close>
@@ -464,24 +494,38 @@ proof (induction rule: cdcl\<^sub>W_OOO_conflict.induct)
     using assms(2) unfolding cdcl\<^sub>W_all_struct_inv_def cdcl\<^sub>W_M_level_inv_def by fast
   with assms(2) cdcl\<^sub>W_OOO_conflict_rule show ?case
      by (auto simp: backtrack_lvl_cut_trail_wrt_clause_get_maximum_level
-      get_maximum_level_cut_trail_wrt_clause
-      add_new_clause_and_update_def dest!: get_maximum_level_exists_lit_of_max_level[of _ \<open>trail T\<close>])
+        get_maximum_level_cut_trail_wrt_clause reduce_trail_wrt_clause_def
+      dest!: get_maximum_level_exists_lit_of_max_level[of _ \<open>trail T\<close>])
 qed
 
-text \<open>We can fully run @{term cdcl\<^sub>W_stgy} or add a clause.\<close>
+text \<open>We can fully run @{term cdcl\<^sub>W_stgy} or add a clause.
+
+Compared to a previous I changed the order and replaced \<^term>\<open>(update_conflicting (Some C)
+       (add_init_cls C (cut_trail_wrt_clause C (trail S) S)))\<close> (like in my thesis) by
+\<^term>\<open>(update_conflicting (Some C) (cut_trail_wrt_clause C (trail S) (add_init_cls C S)))\<close>.
+The motivation behind it is that adding clause first makes it fallback on conflict (with
+backtracking, but it is still a conflict) and, therefore, seems more regular than the opposite order.
+\<close>
 inductive incremental_cdcl\<^sub>W :: "'st \<Rightarrow> 'st \<Rightarrow> bool" for S where
 add_confl:
   "trail S \<Turnstile>asm init_clss S \<Longrightarrow> distinct_mset C \<Longrightarrow> conflicting S = None \<Longrightarrow>
    trail S \<Turnstile>as CNot C \<Longrightarrow>
    full cdcl\<^sub>W_stgy
      (update_conflicting (Some C)
-       (add_init_cls C (cut_trail_wrt_clause C (trail S) S))) T \<Longrightarrow>
+       (cut_trail_wrt_clause C (trail S) (add_init_cls C S))) T \<Longrightarrow>
    incremental_cdcl\<^sub>W S T" |
 add_no_confl:
   "trail S \<Turnstile>asm init_clss S \<Longrightarrow> distinct_mset C \<Longrightarrow> conflicting S = None \<Longrightarrow>
    \<not>trail S \<Turnstile>as CNot C \<Longrightarrow>
    full cdcl\<^sub>W_stgy (add_init_cls C S) T \<Longrightarrow>
    incremental_cdcl\<^sub>W S T"
+
+
+lemma cdcl\<^sub>W_all_struct_inv_add_init_cls:
+  \<open>cdcl\<^sub>W_all_struct_inv (T) \<Longrightarrow> distinct_mset C \<Longrightarrow> cdcl\<^sub>W_all_struct_inv (add_init_cls C T)\<close>
+  by (auto simp: cdcl\<^sub>W_all_struct_inv_def no_strange_atm_def cdcl\<^sub>W_M_level_inv_def
+    distinct_cdcl\<^sub>W_state_def cdcl\<^sub>W_conflicting_def cdcl\<^sub>W_learned_clause_def clauses_def
+    reasons_in_clauses_def all_decomposition_implies_insert_single)
 
 lemma cdcl\<^sub>W_all_struct_inv_add_new_clause_and_update_cdcl\<^sub>W_stgy_inv:
   assumes
@@ -493,16 +537,23 @@ lemma cdcl\<^sub>W_all_struct_inv_add_new_clause_and_update_cdcl\<^sub>W_stgy_in
   shows "cdcl\<^sub>W_stgy_invariant (add_new_clause_and_update C T)"
     (is "cdcl\<^sub>W_stgy_invariant ?T'")
 proof -
-  have "cdcl\<^sub>W_all_struct_inv ?T'"
-    using cdcl\<^sub>W_all_struct_inv_add_new_clause_and_update_cdcl\<^sub>W_all_struct_inv assms by blast
+  let ?S = \<open>add_init_cls C T\<close>
+  let ?T = \<open>(reduce_trail_wrt_clause C ?S)\<close>
+
+  have "cdcl\<^sub>W_all_struct_inv ?S"
+   using assms by (auto simp: cdcl\<^sub>W_all_struct_inv_add_init_cls)
+  then have "cdcl\<^sub>W_all_struct_inv ?T"
+    using cdcl\<^sub>W_all_struct_inv_add_new_clause_and_update_cdcl\<^sub>W_all_struct_inv[of ?S C] assms
+    by auto
   then have
     no_dup_cut_T[simp]: "no_dup (trail (cut_trail_wrt_clause C (trail T) T))" and
     n_d[simp]: "no_dup (trail T)"
     using cdcl\<^sub>W_M_level_inv_decomp(2) cdcl\<^sub>W_all_struct_inv_def inv
     n_dup_no_dup_trail_cut_trail_wrt_clause by blast+
   then have "trail (add_new_clause_and_update C T) \<Turnstile>as CNot C"
-    by (simp add: add_new_clause_and_update_def cut_trail_wrt_clause_CNot_trail
-      cdcl\<^sub>W_M_level_inv_def cdcl\<^sub>W_all_struct_inv_def)
+    by (simp add: cut_trail_wrt_clause_CNot_trail
+      cdcl\<^sub>W_M_level_inv_def cdcl\<^sub>W_all_struct_inv_def add_new_clause_and_update_def
+      reduce_trail_wrt_clause_def)
   obtain MT where
     MT: "trail T = MT @  trail (cut_trail_wrt_clause C (trail T) T)"
     using trail_cut_trail_wrt_clause by blast
@@ -514,67 +565,69 @@ proof -
         "1 \<le> length (trail (cut_trail_wrt_clause C (trail T) T))"
     using cut_trail_wrt_clause_hd_trail_in_or_empty_trail[of "C" T] by auto
   then show ?thesis
-    proof cases
-      case false note C = this(1) and empty_tr = this(2)
-      then have [simp]: "C = {#}"
-        by (simp add: in_CNot_implies_uminus(2) multiset_eqI)
-      show ?thesis
-        using empty_tr unfolding cdcl\<^sub>W_stgy_invariant_def no_smaller_confl_def
-        cdcl\<^sub>W_all_struct_inv_def by (auto simp: add_new_clause_and_update_def)
-    next
-      case not_false note C = this(1) and l = this(2)
-      let ?L = "- lit_of (hd (trail (cut_trail_wrt_clause C (trail T) T)))"
-      have L: "get_level (trail (cut_trail_wrt_clause C (trail T) T)) (-?L)
-        = count_decided (trail (cut_trail_wrt_clause C (trail T) T))"
-        apply (cases "trail (add_init_cls C
-            (cut_trail_wrt_clause C (trail T) T))";
-         cases "hd (trail (cut_trail_wrt_clause C (trail T) T))")
-        using l by (auto split: if_split_asm
-          simp:rev_swap[symmetric] add_new_clause_and_update_def)
+  proof cases
+    case false note C = this(1) and empty_tr = this(2)
+    then have [simp]: "C = {#}"
+      by (simp add: in_CNot_implies_uminus(2) multiset_eqI)
+    show ?thesis
+      using empty_tr unfolding cdcl\<^sub>W_stgy_invariant_def no_smaller_confl_def
+      cdcl\<^sub>W_all_struct_inv_def by (auto simp: add_new_clause_and_update_def
+    reduce_trail_wrt_clause_def)
+  next
+    case not_false note C = this(1) and l = this(2)
+    let ?L = "- lit_of (hd (trail (cut_trail_wrt_clause C (trail T) T)))"
+    have L: "get_level (trail (cut_trail_wrt_clause C (trail T) T)) (-?L)
+      = count_decided (trail (cut_trail_wrt_clause C (trail T) T))"
+      apply (cases "trail (add_init_cls C
+          (cut_trail_wrt_clause C (trail T) T))";
+       cases "hd (trail (cut_trail_wrt_clause C (trail T) T))")
+      using l by (auto split: if_split_asm
+        simp:rev_swap[symmetric] add_new_clause_and_update_def)
 
-      have [simp]: "no_smaller_confl (update_conflicting (Some C)
-        (add_init_cls C (cut_trail_wrt_clause C (trail T) T)))"
-        unfolding no_smaller_confl_def
-      proof (clarify, goal_cases)
-        case (1 M K M' D)
-        then consider
-            (DC) "D = C"
-          | (D_T) "D \<in># clauses T"
-          by (auto simp: clauses_def split: if_split_asm)
-        then show False
-          proof cases
-            case D_T
-            have "no_smaller_confl T"
-              using inv_s unfolding cdcl\<^sub>W_stgy_invariant_def by auto
-            have "trail T = (MT @ M') @ Decided K # M"
-              using MT 1(1) by auto
-            then show False
-              using D_T \<open>no_smaller_confl T\<close> 1(3) unfolding no_smaller_confl_def by blast
-          next
-            case DC note _[simp] = this
-            then have "atm_of (-?L) \<in> atm_of ` (lits_of_l M)"
-              using 1(3) C in_CNot_implies_uminus(2) by blast
-            moreover
-              have "lit_of (hd (M' @ Decided K # [])) = -?L"
-                using l 1(1)[symmetric] inv
-                by (cases M', cases "trail (add_init_cls C
-                    (cut_trail_wrt_clause C (trail T) T))")
-                (auto dest!: arg_cong[of "_ # _" _ hd] simp: hd_append cdcl\<^sub>W_all_struct_inv_def
-                  cdcl\<^sub>W_M_level_inv_def)
-              from arg_cong[OF this, of atm_of]
-              have "atm_of (-?L) \<in> atm_of ` (lits_of_l (M' @ Decided K # []))"
-                by (cases " (M' @ Decided K # [])") auto
-            moreover have "no_dup (trail (cut_trail_wrt_clause C (trail T) T))"
-              using \<open>cdcl\<^sub>W_all_struct_inv ?T'\<close> unfolding cdcl\<^sub>W_all_struct_inv_def
-              cdcl\<^sub>W_M_level_inv_def by (auto simp: add_new_clause_and_update_def)
-            ultimately show False
-              unfolding 1(1)[simplified] by (auto simp: lits_of_def no_dup_def)
-        qed
+    have [simp]: "no_smaller_confl (update_conflicting (Some C)
+      (cut_trail_wrt_clause C (trail T) (add_init_cls C T)))"
+      unfolding no_smaller_confl_def
+    proof (clarify, goal_cases)
+      case (1 M K M' D)
+      then consider
+          (DC) "D = C"
+        | (D_T) "D \<in># clauses T"
+        by (auto simp: clauses_def split: if_split_asm)
+      then show False
+        proof cases
+          case D_T
+          have "no_smaller_confl T"
+            using inv_s unfolding cdcl\<^sub>W_stgy_invariant_def by auto
+          have "trail T = (MT @ M') @ Decided K # M"
+            using MT 1(1) by auto
+          then show False
+            using D_T \<open>no_smaller_confl T\<close> 1(3) unfolding no_smaller_confl_def by blast
+        next
+          case DC note _[simp] = this
+          then have "atm_of (-?L) \<in> atm_of ` (lits_of_l M)"
+            using 1(3) C in_CNot_implies_uminus(2) by blast
+          moreover
+            have "lit_of (hd (M' @ Decided K # [])) = -?L"
+              using l 1(1)[symmetric] inv
+              by (cases M', cases "trail (add_init_cls C
+                  (cut_trail_wrt_clause C (trail T) T))")
+              (auto dest!: arg_cong[of "_ # _" _ hd] simp: hd_append cdcl\<^sub>W_all_struct_inv_def
+                cdcl\<^sub>W_M_level_inv_def)
+            from arg_cong[OF this, of atm_of]
+            have "atm_of (-?L) \<in> atm_of ` (lits_of_l (M' @ Decided K # []))"
+              by (cases " (M' @ Decided K # [])") auto
+          moreover have "no_dup (trail (cut_trail_wrt_clause C (trail T) T))"
+            using \<open>cdcl\<^sub>W_all_struct_inv ?T\<close> unfolding cdcl\<^sub>W_all_struct_inv_def
+            cdcl\<^sub>W_M_level_inv_def by (auto simp: add_new_clause_and_update_def)
+          ultimately show False
+            unfolding 1(1)[simplified] by (auto simp: lits_of_def no_dup_def)
       qed
-      show ?thesis using L C
-        unfolding cdcl\<^sub>W_stgy_invariant_def cdcl\<^sub>W_all_struct_inv_def
-        by (auto simp: add_new_clause_and_update_def get_level_def count_decided_def intro: rev_bexI)
     qed
+    show ?thesis using L C
+      unfolding cdcl\<^sub>W_stgy_invariant_def cdcl\<^sub>W_all_struct_inv_def
+      by (auto simp: add_new_clause_and_update_def get_level_def count_decided_def
+        reduce_trail_wrt_clause_def intro: rev_bexI)
+  qed
 qed
 
 lemma incremental_cdcl\<^sub>W_inv:
@@ -590,22 +643,28 @@ lemma incremental_cdcl\<^sub>W_inv:
   using inc
 proof induction
   case (add_confl C T)
-  let ?T = "(update_conflicting (Some C) (add_init_cls C
-    (cut_trail_wrt_clause C (trail S) S)))"
-  have inv': "cdcl\<^sub>W_all_struct_inv ?T" and inv_s_T: "cdcl\<^sub>W_stgy_invariant ?T"
+  let ?T = "(update_conflicting (Some C) (cut_trail_wrt_clause C (trail S) (add_init_cls C S)))"
+  have \<open>cdcl\<^sub>W_all_struct_inv (add_init_cls C S)\<close>
+    using cdcl\<^sub>W_all_struct_inv_add_init_cls add_confl.hyps(2) inv by auto
+  then have inv': "cdcl\<^sub>W_all_struct_inv ?T" and inv_s_T: "cdcl\<^sub>W_stgy_invariant ?T"
+    using add_confl.hyps(1,2,4)
+    cdcl\<^sub>W_all_struct_inv_add_new_clause_and_update_cdcl\<^sub>W_all_struct_inv[of \<open>add_init_cls C S\<close> C] inv
+     apply (auto simp:  add_new_clause_and_update_def reduce_trail_wrt_clause_def)
     using add_confl.hyps(1,2,4) add_new_clause_and_update_def
-    cdcl\<^sub>W_all_struct_inv_add_new_clause_and_update_cdcl\<^sub>W_all_struct_inv inv apply auto[1]
-    using add_confl.hyps(1,2,4) add_new_clause_and_update_def
-    cdcl\<^sub>W_all_struct_inv_add_new_clause_and_update_cdcl\<^sub>W_stgy_inv inv s_inv by auto
+    cdcl\<^sub>W_all_struct_inv_add_new_clause_and_update_cdcl\<^sub>W_stgy_inv inv s_inv
+    by (auto simp:  add_new_clause_and_update_def reduce_trail_wrt_clause_def)
+
   case 1 show ?case
-     by (metis add_confl.hyps(2,4,5) add_new_clause_and_update_def
-       cdcl\<^sub>W_all_struct_inv_add_new_clause_and_update_cdcl\<^sub>W_all_struct_inv
-       rtranclp_cdcl\<^sub>W_all_struct_inv_inv rtranclp_cdcl\<^sub>W_stgy_rtranclp_cdcl\<^sub>W_restart full_def inv)
+    using add_confl rtranclp_cdcl\<^sub>W_all_struct_inv_inv[of ?T T]
+     rtranclp_cdcl\<^sub>W_stgy_rtranclp_cdcl\<^sub>W_restart[of ?T T] inv'
+    unfolding full_def
+    by auto
 
   case 2 show ?case
-    by (metis inv_s_T add_confl.hyps(2,4,5) add_new_clause_and_update_def
-      cdcl\<^sub>W_all_struct_inv_add_new_clause_and_update_cdcl\<^sub>W_all_struct_inv full_def inv
-      rtranclp_cdcl\<^sub>W_stgy_cdcl\<^sub>W_stgy_invariant)
+    using add_confl rtranclp_cdcl\<^sub>W_all_struct_inv_inv[of ?T T]
+     rtranclp_cdcl\<^sub>W_stgy_rtranclp_cdcl\<^sub>W_restart[of ?T T] inv'
+     inv_s_T rtranclp_cdcl\<^sub>W_stgy_cdcl\<^sub>W_stgy_invariant 
+    unfolding full_def by blast
 
   case 3 show ?case
     using learned_entailed rtranclp_cdcl\<^sub>W_learned_clauses_entailed[of ?T T]  add_confl inv'
